fairness/fin_branch.v
@@ -1,0 +1,63 @@
+From stdpp Require Import base sets.
+From iris.proofmode Require Import tactics.
+From trillium.fairness Require Import
+                         (* locales_helpers comp_utils trace_lookup fairness *)
+                       utils.
+(* TODO: move the needed lemmas *)
+From trillium.fairness.lawyer.obligations Require Import obls_utils.
+
+
+Section ListApprox.
+  Context {A: Type}.
+
+  Definition list_approx (P: A -> Prop) :=
+    { l: list A | forall a, P a -> a ∈ l }. 
+
+  Fixpoint list_approx_repeat (R: A -> A → Prop)
+      (APX: forall a, list_approx (R a))      
+      (n: nat)
+      (a: A)
+      :=
+      match n with
+      | 0 => [a]
+      | S n =>
+          let la := APX a in
+          flat_map (list_approx_repeat R APX n) (proj1_sig la)
+      end.
+
+  Lemma list_approx_repeat_spec (R: A -> A -> Prop) APX n a:
+    forall b, relations.nsteps R n a b -> b ∈ list_approx_repeat R APX n a.
+  Proof using.
+    revert a. induction n.
+    { simpl. intros ??. rewrite nsteps_0. set_solver. }
+    intros ??. rewrite -rel_compose_nsteps_next'.       
+    intros (? & STEP & STEPS). 
+    apply IHn in STEPS. simpl.
+    apply elem_of_list_In. apply in_flat_map. eexists. split.
+    2: eapply elem_of_list_In; eauto.
+    destruct APX. simpl in *. apply elem_of_list_In. eauto.
+  Qed.
+
+End ListApprox.
+
+Section SmallerCardLA.
+  Context {A: Type}.
+  Context {EQDEC: EqDecision A}.
+  Context (P: A -> Prop).
+
+  From trillium.prelude Require Import classical_instances.
+  
+  Local Instance P_PI: forall a, ProofIrrel (P a).
+  Proof using. intros. apply make_proof_irrel. Qed.  
+
+  Lemma list_approx_smaller_card (APX: list_approx P):
+    quantifiers.smaller_card {a | P a} nat.
+  Proof using EQDEC.
+    apply finitary.finite_smaller_card_nat.
+    destruct APX as [??]. 
+    by eapply finitary.in_list_finite.
+  Qed.
+
+End SmallerCardLA.
+
+
