fairness/lawyer/obligations/obligations_resources.v
@@ -2,7 +2,7 @@ From iris.proofmode Require Import tactics.
 From iris.base_logic Require Import own. 
 From iris.algebra Require Import auth gmap gset excl gmultiset big_op mono_nat.
 From trillium.fairness Require Import (* fairness *) locales_helpers utils.
-From trillium.fairness.lawyer Require Import obligations_model. 
+From trillium.fairness.lawyer.obligations Require Import obligations_model. 
 From stdpp Require Import namespaces. 
 From trillium.fairness.lawyer.obligations Require Import obls_utils.
 
